use recursive partition to prove eval_div axiom

src/Experiments/NewPipeline/Arithmetic.v
@@ -1456,7 +1456,39 @@ Module Partition.
       rewrite weight_0 by auto; autorewrite with zsimplify_fast.
       reflexivity.
     Qed.
+
+    Lemma length_recursive_partition n : forall i x,
+      length (recursive_partition n i x) = n.
+    Proof.
+      induction n; cbn [recursive_partition]; [reflexivity | ].
+      intros; distr_length; auto.
+    Qed.
+    Hint Rewrite length_recursive_partition : distr_length.
+
+    (* TODO : move *)
+    Hint Rewrite Nat.sub_0_l : natsimplify.
+
+    (* TODO : remove if this ends up being unused *)
+    Lemma recursive_partition_skipn : forall m n i j x,
+        (m < n)%nat ->
+        (j = i + m)%nat ->
+        skipn m (recursive_partition n i (x / weight i)) = recursive_partition (n-m) j (x / weight j).
+    Proof.
+      induction m; destruct n; intros; subst;
+        repeat match goal with
+               | _ => progress cbn [recursive_partition]
+               | _ => rewrite weight_0 by assumption
+               | _ => rewrite weight_multiples by assumption
+               | _ => rewrite Z.div_div by auto
+               | _ => rewrite Z.mul_div_eq by auto
+               | _ => progress autorewrite with zsimplify_fast natsimplify push_skipn
+               | _ => reflexivity
+               end.
+      erewrite IHm by (auto; omega).
+      repeat (f_equal; try omega).
+    Qed.
   End Partition.
+  Hint Rewrite length_partition length_recursive_partition : distr_length.
 End Partition.
 
 Module Columns.
@@ -3018,9 +3050,24 @@ Module UniformWeight.
   Proof using Type. now cbv [uweight weight]; autorewrite with zsimplify_fast. Qed.
   Lemma uweight_eq_alt lgr (Hr : 0 <= lgr) n : uweight lgr n = (2^lgr)^Z.of_nat n.
   Proof using Type. now rewrite uweight_eq_alt', Z.pow_mul_r by lia. Qed.
+  Lemma uweight_eval_shift lgr (Hr : 0 <= lgr) xs :
+    forall n,
+    length xs = n ->
+    Positional.eval (fun i => uweight lgr (S i)) n xs =
+    (uweight lgr 1) * Positional.eval (uweight lgr) n xs.
+  Proof.
+    induction xs using rev_ind; destruct n; distr_length;
+      intros; [cbn; ring | ].
+    rewrite !Positional.eval_snoc with (n:=n) by distr_length.
+    rewrite IHxs, !uweight_eq_alt by omega.
+    autorewrite with push_Zof_nat push_Zpow.
+    rewrite !Z.pow_succ_r by auto using Nat2Z.is_nonneg.
+    ring.
+  Qed.
 End UniformWeight.
 
 Module WordByWordMontgomery.
+  Import Partition.
   Section with_args.
     Context (lgr : Z)
             (m : Z).
@@ -3116,7 +3163,7 @@ Module WordByWordMontgomery.
     Let R := (r^Z.of_nat R_numlimbs).
     Transparent T.
     Definition small {n} (v : T n) : Prop
-      := v = Partition.partition weight n (eval v).
+      := v = partition weight n (eval v).
     Context (small_N : small N)
             (N_lt_R : eval N < R)
             (N_nz : 0 < eval N)
@@ -3140,18 +3187,18 @@ Module WordByWordMontgomery.
     Lemma length_small {n v} : @small n v -> length v = n.
     Proof using Type. clear; cbv [small]; intro H; rewrite H; autorewrite with distr_length; reflexivity. Qed.
 
-    Let partition_Proper := (@Partition.partition_Proper _ wprops).
+    Let partition_Proper := (@partition_Proper _ wprops).
     Local Existing Instance partition_Proper.
     Lemma eval_nonzero n A : @small n A -> nonzero A = 0 <-> @eval n A = 0.
     Proof using lgr_big.
       clear -lgr_big partition_Proper.
       cbv [nonzero eval small]; intro Heq.
       do 2 rewrite Heq.
-      rewrite !Partition.eval_partition, Z.mod_mod by auto.
+      rewrite !eval_partition, Z.mod_mod by auto.
       generalize (Positional.eval weight n A); clear Heq A.
       induction n as [|n IHn].
       { cbn; rewrite weight_0 by auto; intros; autorewrite with zsimplify_const; omega. }
-      { intro; rewrite Partition.partition_step.
+      { intro; rewrite partition_step.
         rewrite fold_right_snoc, Z.lor_comm, <- fold_right_push, Z.lor_eq_0_iff by auto using Z.lor_assoc.
         assert (Heq : Z.equiv_modulo (weight n) (z mod weight (S n)) (z mod (weight n))).
         { cbv [Z.equiv_modulo].
@@ -3214,10 +3261,34 @@ Module WordByWordMontgomery.
     Qed.
     Local Lemma small_zero : forall n, small (@zero n).
     Proof using Type.
-      etransitivity; [ eapply Positional.zeros_ext_map | rewrite eval_zero ]; cbv [Partition.partition]; cbn; try reflexivity; autorewrite with distr_length; reflexivity.
+      etransitivity; [ eapply Positional.zeros_ext_map | rewrite eval_zero ]; cbv [partition]; cbn; try reflexivity; autorewrite with distr_length; reflexivity.
     Qed.
     Local Hint Immediate small_zero.
-    Local Axiom eval_div : forall n v, small v -> eval (fst (@divmod n v)) = eval v / r.
+
+    (* TODO : relocate? *)
+    Lemma weight_1 : weight 1 = r.
+    Proof.
+      clear - lgr_big. subst r.
+      rewrite UniformWeight.uweight_eq_alt by omega.
+      cbn; ring.
+    Qed.
+
+    Lemma eval_div : forall n v, small v -> eval (fst (@divmod n v)) = eval v / r.
+    Proof.
+      pose proof r_big as r_big.
+      clear - r_big lgr_big; autounfold with loc; intros.
+      repeat match goal with
+             | _ => progress cbn [Rows.divmod fst recursive_partition tl]
+             | H : _ = partition _ _ _ |- _ => rewrite H; clear H
+             | _ => rewrite recursive_partition_equiv by auto using UniformWeight.uwprops
+             | _ => progress rewrite weight_0, weight_1 by auto;
+                      autorewrite with zsimplify_fast
+             | _ => rewrite Positional.eval_cons by distr_length
+             | _ => rewrite UniformWeight.uweight_eval_shift by distr_length
+             end.
+      autorewrite with zsimplify.
+      reflexivity.
+    Qed.
     Local Axiom eval_mod : forall n v, small v -> snd (@divmod n v) = eval v mod r.
     Local Axiom small_div : forall n v, small v -> small (fst (@divmod n v)).
     Local Lemma eval_scmul: forall n a v, small v -> 0 <= a < r -> 0 <= eval v < r^Z.of_nat n -> eval (@scmul n a v) = a * eval v.
@@ -3264,7 +3335,7 @@ Module WordByWordMontgomery.
       clear -lgr_big Ha Hb.
       autounfold with loc in *; destruct (zerop n); subst.
       { destruct a as [| ? [|] ], b; cbn; try omega.
-        cbv [Partition.partition seq eval map] in Ha.
+        cbv [partition seq eval map] in Ha.
         cbn in Ha.
         rewrite (weight_0 wprops) in *.
         rewrite Z.add_with_get_carry_full_mod.
@@ -3530,7 +3601,7 @@ Module WordByWordMontgomery.
 
         Lemma fst_redc_body
           : (eval (fst (redc_body A_S))) = eval (fst A_S) / r.
-        Proof using small_S small_A S_bound.
+        Proof using small_S small_A S_bound lgr_big.
           destruct A_S; simpl; repeat autounfold with word_by_word_montgomery; simpl.
           autorewrite with push_mont_eval.
           reflexivity.
@@ -3862,7 +3933,7 @@ Module WordByWordMontgomery.
     Let r := 2^bitwidth.
     Local Notation weight := (UniformWeight.uweight bitwidth).
     Local Notation eval := (@eval bitwidth n).
-    Let m_enc := Partition.partition weight n m.
+    Let m_enc := partition weight n m.
     Local Coercion Z.of_nat : nat >-> Z.
     Context (r' : Z)
             (m' : Z)
@@ -3916,7 +3987,7 @@ Module WordByWordMontgomery.
              | _ => lia
              | _ => exact small_m_enc
              | [ H : small ?x |- context[eval ?x] ]
-               => rewrite H; cbv [eval]; rewrite Partition.eval_partition by auto
+               => rewrite H; cbv [eval]; rewrite eval_partition by auto
              | [ |- context[weight _] ] => rewrite UniformWeight.uweight_eq_alt by auto with omega
              | _=> progress Z.rewrite_mod_small
              | _ => progress Z.zero_bounds
@@ -3947,7 +4018,7 @@ Module WordByWordMontgomery.
         t_fin.
     Qed.
 
-    Definition onemod : list Z := Partition.partition weight n 1.
+    Definition onemod : list Z := partition weight n 1.
 
     Definition onemod_correct : eval onemod = 1 /\ valid onemod.
     Proof using n_nz m_big bitwidth_big.
@@ -3955,7 +4026,7 @@ Module WordByWordMontgomery.
       cbv [valid small onemod eval]; autorewrite with push_eval; t_fin.
     Qed.
 
-    Definition R2mod : list Z := Partition.partition weight n ((r^n * r^n) mod m).
+    Definition R2mod : list Z := partition weight n ((r^n * r^n) mod m).
 
     Definition R2mod_correct : eval R2mod mod m = (r^n*r^n) mod m /\ valid R2mod.
     Proof using n_nz m_small m_big m'_correct bitwidth_big.
@@ -4010,7 +4081,7 @@ Module WordByWordMontgomery.
     Qed.
 
     Definition encodemod (v : Z) : list Z
-      := mulmod (Partition.partition weight n v) R2mod.
+      := mulmod (partition weight n v) R2mod.
 
     Local Ltac t_valid v :=
       cbv [valid]; repeat apply conj;
@@ -4104,7 +4175,7 @@ Module WordByWordMontgomery.
     Lemma to_bytesmod_correct
       : (forall a (_ : valid a), Positional.eval (UniformWeight.uweight 8) (bytes_n bitwidth 1 n) (to_bytesmod a)
                                  = eval a mod m)
-        /\ (forall a (_ : valid a), to_bytesmod a = Partition.partition (UniformWeight.uweight 8) (bytes_n bitwidth 1 n) (eval a mod m)).
+        /\ (forall a (_ : valid a), to_bytesmod a = partition (UniformWeight.uweight 8) (bytes_n bitwidth 1 n) (eval a mod m)).
     Proof using n_nz m_small bitwidth_big.
       clear -n_nz m_small bitwidth_big.
       generalize (@length_small bitwidth n);
